c_stubs/tls13_io_karamel.h
@@ -10,26 +10,4 @@ TLS13_IO_channel tls13_io_channel_from_fd(int fd);
 
 void tls13_io_channel_free(TLS13_IO_channel ch);
 
-typedef struct option__TLS13_IO_channel_s option__TLS13_IO_channel;
-
-option__TLS13_IO_channel TLS13_IO_connect_tcp(
-    uint8_t *hostname,
-    size_t hostname_len,
-    uint16_t port,
-    void *hostname_bytes);
-
-size_t TLS13_IO_read(
-    TLS13_IO_channel ch,
-    uint8_t *out,
-    size_t max_len,
-    void *old);
-
-size_t TLS13_IO_write(
-    TLS13_IO_channel ch,
-    uint8_t *buf,
-    size_t len,
-    void *bytes);
-
-void TLS13_IO_close(TLS13_IO_channel ch);
-
 #endif
